18/09/17　無限降下法の他に、anyを使った定理を証明

program/InfiniteDescent.thy
@@ -2,17 +2,37 @@ theory InfiniteDescent
 imports Main
 begin
 
+
 theorem infinite_descent [simp]:
-  "(\<forall>n. P(n) \<longrightarrow> (\<exists>m. m<n\<and>P(m))) \<longrightarrow> (\<forall>n::nat. \<not>P(n))"
-    apply (metis ex_least_nat_le gr_implies_not0)
-    done
+  "\<forall>P. (\<forall>n. P n  \<longrightarrow> (\<exists>m. m<n \<and> P m)) \<longrightarrow> (\<forall>n::nat. \<not>P n)"
+  (* sledgehammer *)
+  apply (metis ex_least_nat_le gr_implies_not0)
+  done
 
 theorem infinite_descent2 [simp]:
-  "(\<forall>P. (\<forall>n. P(n+1) \<longrightarrow> (\<exists>m::nat. m<n+1 \<and> P(m))) \<longrightarrow> \<not>P(0) \<longrightarrow> (\<forall>n::nat. \<not>P(n)))"
-    (* sledgehammer *)
-    apply (metis Suc_eq_plus1 Suc_leI ex_least_nat_less not_le)
-    done
+  "\<forall>P. (\<forall>n. P(n+1) \<longrightarrow> (\<exists>m::nat. m<n+1 \<and> P m)) \<longrightarrow> \<not>P 0 \<longrightarrow> (\<forall>n::nat. \<not>P n)"
+  (* sledgehammer *)
+  apply (metis Suc_eq_plus1 Suc_leI ex_least_nat_less not_le)
+  done
 
+
+term "[]"
+term "(#)"
+term False
+term fst
+term "(@)"
+term "-1"
+value "add (Suc (Suc 0)) (Suc 0)"
+
+primrec any :: "('a\<Rightarrow>bool) \<Rightarrow> 'a list \<Rightarrow> bool" where
+  "any p [] = False" |
+  "any p (x # xs) = (p x | any p xs)"
+
+lemma any1 [simp]:
+  "\<forall>P. any P (xs@ys) \<longrightarrow> (any P xs) | (any P ys)"
+  apply (induction xs)
+  apply simp
+  apply simp
+  done
 
 end
-
